Include scope in signature, add spec/model to lean_meta standalone

build-debug/out/lean/Logos.lean
@@ -102,7 +102,9 @@ inductive Term : Type where
   | USort : eo_lit_Nat -> Term
   | UConst : eo_lit_Nat -> Term -> Term
   | not : Term
+  | or : Term
   | and : Term
+  | imp : Term
   | eq : Term
 
 deriving Repr, DecidableEq, Inhabited, Ord
@@ -181,6 +183,12 @@ partial def __eo_eq : Term -> Term -> Term
   | t, s => (Term.Boolean (eo_lit_teq s t))
 
 
+partial def __eo_prog_scope : Term -> Proof -> Term
+  | Term.Stuck , _  => Term.Stuck
+  | F, (Proof.pf G) => (Term.Apply (Term.Apply Term.imp F) G)
+  | _, _ => Term.Stuck
+
+
 partial def __eo_prog_contra : Proof -> Proof -> Term
   | (Proof.pf F), (Proof.pf (Term.Apply Term.not __eo_lv_F_2)) => (__eo_requires (__eo_eq F __eo_lv_F_2) (Term.Boolean true) (Term.Boolean false))
   | _, _ => Term.Stuck
@@ -239,6 +247,7 @@ deriving Repr, Inhabited
 /-
 -/
 inductive CRule : Type where
+  | scope : CRule
   | contra : CRule
   | symm : CRule
 
@@ -305,9 +314,10 @@ def __eo_cmd_step_proven (S : CState) : CRule -> CArgList -> CIndexList -> Term
   | r, args, premises => Term.Stuck
 
 
-def __eo_cmd_step_pop_proven (S : CState) (r : CRule) (args : CArgList) : Term -> CIndexList -> Term
-  | Term.Stuck , _  => Term.Stuck
-  | A, premises => Term.Stuck
+def __eo_cmd_step_pop_proven (S : CState) : CRule -> CArgList -> Term -> CIndexList -> Term
+  | _ , _ , Term.Stuck , _  => Term.Stuck
+  | CRule.scope, CArgList.nil, A, (CIndexList.cons n1 CIndexList.nil) => (__eo_prog_scope A (Proof.pf (__eo_state_proven_nth S n1)))
+  | r, args, A, premises => Term.Stuck
 
 
 def __eo_invoke_cmd_step_pop (s : CState) : CState -> CRule -> CArgList -> CIndexList -> CState
@@ -329,17 +339,28 @@ def __eo_invoke_cmd_list (S : CState) : CCmdList -> CState
   | (CCmdList.cons c cmds) => (__eo_invoke_cmd_list (__eo_invoke_cmd S c) cmds)
 
 
-def __eo_invoke_cmd_list_assuming (S : CState) : Term -> CCmdList -> CState
-  | (Term.Apply (Term.Apply Term.and F) as), cs => (__eo_invoke_cmd_list_assuming (CState.cons (CStateObj.assume F) S) as cs)
-  | (Term.Boolean true), cs => (__eo_invoke_cmd_list S cs)
-  | as, cs => CState.Stuck
-
-
 def __eo_state_is_refutation (s : CState) : eo_lit_Bool :=
   (__eo_state_is_closed (__eo_invoke_cmd_check_proven s (Term.Boolean false)))
 
+def __eo_invoke_assume_list (S : CState) : Term -> CState
+  | (Term.Apply (Term.Apply Term.and F) as) => (CState.cons (CStateObj.assume F) (__eo_invoke_assume_list S as))
+  | (Term.Boolean true) => S
+  | as => CState.Stuck
+
+
+def __eo_state_to_formula_rec : CState -> Term -> Term
+  | _ , Term.Stuck  => Term.Stuck
+  | (CState.cons (CStateObj.assume F) s), (Term.Apply (Term.Apply Term.imp F1) (Term.Apply (Term.Apply Term.imp F2) F3)) => (Term.Apply (Term.Apply Term.imp (Term.Apply (Term.Apply Term.and F) F1)) (Term.Apply (Term.Apply Term.imp F2) F3))
+  | (CState.cons (CStateObj.assume_push F) s), (Term.Apply (Term.Apply Term.imp F1) (Term.Apply (Term.Apply Term.imp F2) F3)) => (Term.Apply (Term.Apply Term.imp F1) (Term.Apply (Term.Apply Term.imp (Term.Apply (Term.Apply Term.and F) F2)) F3))
+  | (CState.cons (CStateObj.proven F) s), (Term.Apply (Term.Apply Term.imp F1) (Term.Apply (Term.Apply Term.imp F2) F3)) => (Term.Apply (Term.Apply Term.imp F1) (Term.Apply (Term.Apply Term.imp F2) (Term.Apply (Term.Apply Term.and F) F3)))
+  | s, F => Term.Stuck
+
+
+def __eo_state_to_formula (s : CState) : Term :=
+  (__eo_state_to_formula_rec s (Term.Apply (Term.Apply Term.imp (Term.Boolean true)) (Term.Apply (Term.Apply Term.imp (Term.Boolean true)) (Term.Boolean true))))
+
 def __eo_checker_is_refutation : Term -> CCmdList -> eo_lit_Bool
-  | as, cs => (__eo_state_is_refutation (__eo_invoke_cmd_list_assuming CState.nil as cs))
+  | as, cs => (__eo_state_is_refutation (__eo_invoke_cmd_list (__eo_invoke_assume_list CState.nil as) cs))
 
 
 
