plugins/lean_meta/lean_meta.lean
@@ -171,6 +171,249 @@ macro_rules
 
 end SmtEval
 
+
+namespace Smtm
+
+/- SMT literal evaluation defined -/
+
+abbrev smt_lit_Bool := SmtEval.smt_lit_Bool
+abbrev smt_lit_Int := SmtEval.smt_lit_Int
+abbrev smt_lit_Rat := SmtEval.smt_lit_Rat
+abbrev smt_lit_String := SmtEval.smt_lit_String
+abbrev smt_lit_RegLan := String --FIXME
+
+def smt_lit_ite {T : Type} (c : smt_lit_Bool) (t e : T) : T :=
+  if c then t else e
+abbrev smt_lit_not := SmtEval.smt_lit_not
+abbrev smt_lit_and := SmtEval.smt_lit_and
+abbrev smt_lit_iff := SmtEval.smt_lit_iff
+abbrev smt_lit_or := SmtEval.smt_lit_or
+abbrev smt_lit_xor := SmtEval.smt_lit_xor
+abbrev smt_lit_zplus := SmtEval.smt_lit_zplus
+abbrev smt_lit_zmult := SmtEval.smt_lit_zmult
+abbrev smt_lit_zneg := SmtEval.smt_lit_zneg
+abbrev smt_lit_zeq := SmtEval.smt_lit_zeq
+abbrev smt_lit_zleq := SmtEval.smt_lit_zleq
+abbrev smt_lit_zlt := SmtEval.smt_lit_zlt
+abbrev smt_lit_div_total := SmtEval.smt_lit_div_total
+abbrev smt_lit_mod_total := SmtEval.smt_lit_mod_total
+abbrev smt_lit_zexp_total := SmtEval.smt_lit_zexp_total
+abbrev smt_lit_int_pow2 := SmtEval.smt_lit_int_pow2
+abbrev smt_lit_piand := SmtEval.smt_lit_piand
+abbrev smt_lit_mk_rational := SmtEval.smt_lit_mk_rational
+abbrev smt_lit_qplus := SmtEval.smt_lit_qplus
+abbrev smt_lit_qmult := SmtEval.smt_lit_qmult
+abbrev smt_lit_qneg := SmtEval.smt_lit_qneg
+abbrev smt_lit_qeq := SmtEval.smt_lit_qeq
+abbrev smt_lit_qleq := SmtEval.smt_lit_qleq
+abbrev smt_lit_qlt := SmtEval.smt_lit_qlt
+abbrev smt_lit_qdiv_total := SmtEval.smt_lit_qdiv_total
+abbrev smt_lit_to_int := SmtEval.smt_lit_to_int
+abbrev smt_lit_to_real := SmtEval.smt_lit_to_real
+abbrev smt_lit_str_len := SmtEval.smt_lit_str_len
+abbrev smt_lit_str_concat := SmtEval.smt_lit_str_concat
+abbrev smt_lit_str_substr := SmtEval.smt_lit_str_substr
+abbrev smt_lit_str_indexof := SmtEval.smt_lit_str_indexof
+abbrev smt_lit_str_to_code := SmtEval.smt_lit_str_to_code
+abbrev smt_lit_str_from_code := SmtEval.smt_lit_str_from_code
+
+abbrev smt_lit_bit := SmtEval.smt_lit_bit
+abbrev smt_lit_msb := SmtEval.smt_lit_msb
+abbrev smt_lit_binary_and := SmtEval.smt_lit_binary_and
+abbrev smt_lit_binary_or := SmtEval.smt_lit_binary_or
+abbrev smt_lit_binary_xor := SmtEval.smt_lit_binary_xor
+abbrev smt_lit_binary_not := SmtEval.smt_lit_binary_not
+abbrev smt_lit_binary_max := SmtEval.smt_lit_binary_max
+abbrev smt_lit_binary_uts := SmtEval.smt_lit_binary_uts
+abbrev smt_lit_binary_concat := SmtEval.smt_lit_binary_concat
+abbrev smt_lit_binary_extract := SmtEval.smt_lit_binary_extract
+
+abbrev smt_lit_Nat := SmtEval.smt_lit_Nat
+abbrev smt_lit_int_to_nat := SmtEval.smt_lit_int_to_nat
+abbrev smt_lit_nat_to_int := SmtEval.smt_lit_nat_to_int
+abbrev smt_lit_nateq := SmtEval.smt_lit_nateq
+
+-- SMT Beyond Eunoia
+
+def smt_lit_streq : smt_lit_String -> smt_lit_String -> smt_lit_Bool
+  | x, y => decide (x = y)
+
+def smt_lit_int_log2 : smt_lit_Int -> smt_lit_Int
+  | _ => 0 -- FIXME
+
+def smt_lit_str_lt : smt_lit_String -> smt_lit_String -> smt_lit_Bool
+  | _, _ => false -- FIXME
+def smt_lit_str_from_int : smt_lit_Int -> smt_lit_String
+  | _ => "" -- FIXME
+def smt_lit_str_to_int : smt_lit_String -> smt_lit_Int
+  | _ => 0 -- FIXME
+def smt_lit_str_to_upper : smt_lit_String -> smt_lit_String
+  | _ => "" -- FIXME
+def smt_lit_str_to_lower : smt_lit_String -> smt_lit_String
+  | _ => "" -- FIXME
+def smt_lit_str_update : smt_lit_String -> smt_lit_Int -> smt_lit_String -> smt_lit_String
+  | _, _, _ => "" -- FIXME
+def smt_lit_str_rev : smt_lit_String -> smt_lit_String
+  | _ => "" -- FIXME
+def smt_lit_str_replace : smt_lit_String -> smt_lit_String -> smt_lit_String -> smt_lit_String
+  | _, _, _ => "" -- FIXME
+def smt_lit_str_replace_all : smt_lit_String -> smt_lit_String -> smt_lit_String -> smt_lit_String
+  | _, _, _ => "" -- FIXME
+def smt_lit_str_contains : smt_lit_String -> smt_lit_String -> smt_lit_Bool
+  | _, _ => false -- FIXME
+def smt_lit_str_to_re : smt_lit_String -> smt_lit_RegLan
+  | _ => "" -- FIXME
+def smt_lit_re_mult : smt_lit_RegLan -> smt_lit_RegLan
+  | _ => "" -- FIXME
+def smt_lit_re_plus : smt_lit_RegLan -> smt_lit_RegLan
+  | _ => "" -- FIXME
+def smt_lit_re_comp : smt_lit_RegLan -> smt_lit_RegLan
+  | _ => "" -- FIXME
+def smt_lit_re_concat : smt_lit_RegLan -> smt_lit_RegLan -> smt_lit_RegLan
+  | _, _ => "" -- FIXME
+def smt_lit_re_inter : smt_lit_RegLan -> smt_lit_RegLan -> smt_lit_RegLan
+  | _, _ => "" -- FIXME
+def smt_lit_re_diff : smt_lit_RegLan -> smt_lit_RegLan -> smt_lit_RegLan
+  | _, _ => "" -- FIXME
+def smt_lit_re_union : smt_lit_RegLan -> smt_lit_RegLan -> smt_lit_RegLan
+  | _, _ => "" -- FIXME
+def smt_lit_re_range : smt_lit_String -> smt_lit_String -> smt_lit_RegLan
+  | _, _ => "" -- FIXME
+def smt_lit_str_in_re : smt_lit_String -> smt_lit_RegLan -> smt_lit_Bool
+  | _, _ => false -- FIXME
+def smt_lit_str_indexof_re : smt_lit_String -> smt_lit_RegLan -> smt_lit_Int -> smt_lit_Int
+  | _, _, _ => 0 -- FIXME
+def smt_lit_str_replace_re : smt_lit_String -> smt_lit_RegLan -> smt_lit_String -> smt_lit_String
+  | _, _, _ => "" -- FIXME
+def smt_lit_str_replace_re_all : smt_lit_String -> smt_lit_RegLan -> smt_lit_String -> smt_lit_String
+  | _, _, _ => "" -- FIXME
+def smt_lit_re_allchar : smt_lit_RegLan := "" --FIXME
+def smt_lit_re_none : smt_lit_RegLan := "" --FIXME
+def smt_lit_re_all : smt_lit_RegLan := "" --FIXME
+
+-- Partial semantics
+
+def smt_lit_qdiv_by_zero_id : smt_lit_Int := -1
+def smt_lit_div_by_zero_id : smt_lit_Int := -2
+def smt_lit_mod_by_zero_id : smt_lit_Int := -3
+def smt_lit_wrong_apply_sel_id : smt_lit_Int := -4
+
+mutual
+
+/- 
+SMT-LIB types.
+-/
+inductive SmtType : Type where
+  | None : SmtType
+  | Bool : SmtType
+  | Int : SmtType
+
+deriving Repr, DecidableEq, Inhabited
+
+/- 
+SMT-LIB terms.
+-/
+inductive SmtTerm : Type where
+  | None : SmtTerm
+  | Boolean : smt_lit_Bool -> SmtTerm
+  | Numeral : smt_lit_Int -> SmtTerm
+  | Apply : SmtTerm -> SmtTerm -> SmtTerm
+  | eq : SmtTerm
+  | not : SmtTerm
+  | or : SmtTerm
+  | and : SmtTerm
+  | imp : SmtTerm
+
+deriving Repr, DecidableEq, Inhabited
+
+/- 
+SMT-LIB values.
+-/
+inductive SmtValue : Type where
+  | NotValue : SmtValue
+  | Boolean : smt_lit_Bool -> SmtValue
+  | Numeral : smt_lit_Int -> SmtValue
+
+deriving Repr, DecidableEq, Inhabited
+
+end
+
+/-
+SMT-LIB model
+-/
+abbrev SmtModel := Int -- FIXME
+
+
+/- Type equality -/
+def smt_lit_Teq : SmtType -> SmtType -> smt_lit_Bool
+  | x, y => decide (x = y)
+/- Value equality -/
+def smt_lit_veq : SmtValue -> SmtValue -> smt_lit_Bool
+  | x, y => decide (x = y)
+
+/- Definition of SMT-LIB model semantics -/
+
+mutual
+
+def __smtx_typeof_value : SmtValue -> SmtType
+  | (SmtValue.Boolean b) => SmtType.Bool
+  | (SmtValue.Numeral n) => SmtType.Int
+  | v => SmtType.None
+
+
+def __smtx_model_eval_eq (t1 : SmtValue) (t2 : SmtValue) : SmtValue :=
+  (smt_lit_ite (smt_lit_Teq (__smtx_typeof_value t1) (__smtx_typeof_value t2)) (smt_lit_ite (smt_lit_Teq (__smtx_typeof_value t1) SmtType.None) SmtValue.NotValue (SmtValue.Boolean (smt_lit_veq t1 t2))) SmtValue.NotValue)
+
+def __smtx_model_eval_not : SmtValue -> SmtValue
+  | (SmtValue.Boolean x1) => (SmtValue.Boolean (smt_lit_not x1))
+  | t1 => SmtValue.NotValue
+
+
+def __smtx_model_eval_or : SmtValue -> SmtValue -> SmtValue
+  | (SmtValue.Boolean x1), (SmtValue.Boolean x2) => (SmtValue.Boolean (smt_lit_or x1 x2))
+  | t1, t2 => SmtValue.NotValue
+
+
+def __smtx_model_eval_and : SmtValue -> SmtValue -> SmtValue
+  | (SmtValue.Boolean x1), (SmtValue.Boolean x2) => (SmtValue.Boolean (smt_lit_and x1 x2))
+  | t1, t2 => SmtValue.NotValue
+
+
+def __smtx_model_eval_imp (x1 : SmtValue) (x2 : SmtValue) : SmtValue :=
+  (__smtx_model_eval_or (__smtx_model_eval_not x1) x2)
+
+def __smtx_model_eval (M : SmtModel) : SmtTerm -> SmtValue
+  | (SmtTerm.Boolean b) => (SmtValue.Boolean b)
+  | (SmtTerm.Numeral n) => (SmtValue.Numeral n)
+  | (SmtTerm.Apply SmtTerm.not x1) => (__smtx_model_eval_not (__smtx_model_eval M x1))
+  | (SmtTerm.Apply (SmtTerm.Apply SmtTerm.and x1) x2) => (__smtx_model_eval_and (__smtx_model_eval M x1) (__smtx_model_eval M x2))
+  | (SmtTerm.Apply (SmtTerm.Apply SmtTerm.imp x1) x2) => (__smtx_model_eval_imp (__smtx_model_eval M x1) (__smtx_model_eval M x2))
+  | (SmtTerm.Apply (SmtTerm.Apply SmtTerm.eq x1) x2) => (__smtx_model_eval_eq (__smtx_model_eval M x1) (__smtx_model_eval M x2))
+  | x1 => SmtValue.NotValue
+
+
+
+
+end
+
+/-
+SMT interpretation is satisfiability, i.e. the existence of a model
+interpreting the free constants.
+-/
+inductive smt_interprets : SmtTerm -> Bool -> Prop
+  | intro_true  (t : SmtTerm) :
+      (exists M : SmtModel, (__smtx_model_eval M t) = (SmtValue.Boolean true)) ->
+      smt_interprets t true
+  | intro_false (t : SmtTerm) :
+      (forall M : SmtModel, (__smtx_model_eval M t) = (SmtValue.Boolean false))->
+      smt_interprets t false
+
+/- FIXME inductive smt_model_well_typed : SmtModel -> Prop, based on smt axiom -/
+
+/- ---------------------------------------------- -/
+
+end Smtm
+
 namespace Eo
 
 /- Eunoia literal evaluation defined -/
@@ -357,3 +600,96 @@ def logos_invoke_cmd (s : CState) (c :CCmd) : CState := (__eo_invoke_cmd s c)
 def logos_state_is_refutation (s : CState) : eo_lit_Bool := (__eo_state_is_refutation s)
 
 end Eo
+
+
+open Eo
+open Smtm
+
+/- Definition of refutation -/
+
+inductive eo_is_refutation : Term -> CCmdList -> Prop
+  | intro (F : Term) (c : CCmdList) : 
+    (__eo_checker_is_refutation F c) = true -> (eo_is_refutation F c)
+
+
+/-
+A definition of terms in the object language.
+This is to be defined externally.
+-/
+abbrev Object_Term := SmtTerm
+
+/-
+A predicate defining a relation on terms in the object language and Booleans
+such that (s,b) is true if s evaluates to b.
+This is to be defined externally.
+-/
+abbrev obj_interprets := smt_interprets
+
+
+/-
+Definitions for eo_is_obj
+-/
+mutual
+
+def __eo_to_smt_type : Term -> SmtType
+  | T => SmtType.None
+
+
+def __eo_to_smt : Term -> SmtTerm
+  | y => SmtTerm.None
+
+
+end 
+
+/-
+An inductive predicate defining the correspondence between Eunoia terms
+and terms in the object language.
+(t,s) is true if the Eunoia term represents a term s in the object language.
+This is to be custom defined in the Eunoia-to-Lean compiler based on the
+target definition of Object_Term.
+-/
+inductive eo_is_obj : Term -> Object_Term -> Prop
+  | intro (x : Term) : eo_is_obj x (__eo_to_smt x)
+
+
+/-
+A predicate defining when a Eunoia term corresponds to an object term that
+evaluates to true or false.
+(t,b) is true if t is a Eunoia term corresponding to an object term that
+evaluates to b.
+-/
+def eo_interprets (t : Term) (b : Bool) : Prop :=
+  exists (s : Object_Term), (eo_is_obj t s) /\ (obj_interprets s b)
+
+/- The theorem statements -/
+
+/- correctness theorem for __eo_prog_scope -/
+theorem correct___eo_prog_scope (x1 x2 : Term) :
+  (eo_interprets x2 true) ->
+  (Not (eo_interprets (__eo_prog_scope x1 (Proof.pf x2)) false)) :=
+by
+  sorry
+
+/- correctness theorem for __eo_prog_contra -/
+theorem correct___eo_prog_contra (x1 x2 : Term) :
+  (eo_interprets x1 true) ->
+  (eo_interprets x2 true) ->
+  (Not (eo_interprets (__eo_prog_contra (Proof.pf x1) (Proof.pf x2)) false)) :=
+by
+  sorry
+
+/- correctness theorem for __eo_prog_symm -/
+theorem correct___eo_prog_symm (x1 : Term) :
+  (eo_interprets x1 true) ->
+  (Not (eo_interprets (__eo_prog_symm (Proof.pf x1)) false)) :=
+by
+  sorry
+
+
+
+/- correctness theorem for the checker -/
+theorem correct___eo_is_refutation (F : Term) (pf : CCmdList) :
+  (eo_is_refutation F pf) ->
+  (eo_interprets F false) :=
+by
+  sorry
